wip

src/Thread.v
@@ -38,34 +38,30 @@ Import RecordSetNotations.
 
 Require Import
         Types
-        Utils.
+        Utils
+        Decision.
 
 Local Open Scope list.
 Local Open Scope itree_scope.
 Local Open Scope monad_scope.
 Local Open Scope record_set.
 
-Definition instruction_id_t := id_t.
-Definition mem_read_id_t := id_t.
-Definition mem_write_id_t := id_t.
-
-Module Denote (Arc : ArcSig).
+Module Make (Arc : ArcSig).
   Variant threadE : Type -> Type :=
-  | ThEInsFetchAndDecode : threadE Arc.InsSem.ast
-  | ThEInsNextLocs : threadE (list instruction_id_t)
+  | ThEFetchAndDecodeOrRestart : threadE (list instruction_id_t * Arc.InsSem.ast)
   | ThEFinishIns : threadE unit
   | ThERegAccess : forall A, Arc.InsSem.regE A -> threadE A
   (** Load events *)
-  | ThEInitMemLoadOps : Arc.mem_slc -> threadE (list mem_read_id_t)
+  | ThEInitMemLoadOps : mem_slc -> threadE (list mem_read_id_t)
   (* [ThESatMemLoadOpForwarding] returns a bool that indicates if the read
      was fully satisfied, and a list of iids that should be restarted. *)
-  | ThESatMemLoadOpForwarding : mem_read_id_t -> threadE (bool * list mem_write_id_t)
+  | ThESatMemLoadOpForwarding : mem_read_id_t -> threadE (bool * list instruction_id_t)
   (* [ThESatMemLoadOpStorage] returns a list of iids that should be restarted. *)
-  | ThESatMemLoadOpStorage : mem_read_id_t -> threadE (list mem_write_id_t)
-  | ThECompleteLoadOps : threadE Arc.mem_slc_val
+  | ThESatMemLoadOpStorage : mem_read_id_t -> threadE (list instruction_id_t)
+  | ThECompleteLoadOps : threadE mem_slc_val
   (** Store events *)
-  | ThEInitMemStoreOpFps : Arc.mem_slc -> threadE unit
-  | ThEInstaMemStoreOpVals : Arc.mem_slc_val -> threadE unit
+  | ThEInitMemStoreOpFps : mem_slc -> threadE unit
+  | ThEInstaMemStoreOpVals : mem_slc_val -> threadE unit
   | ThECommitStoreInstruction : threadE (list mem_write_id_t)
   (* [ThEPropagateStoreOp] returns a list of iids that should be restarted. *)
   | ThEPropagateStoreOp : mem_write_id_t -> threadE (list instruction_id_t)
@@ -77,20 +73,21 @@ Module Denote (Arc : ArcSig).
 
   Definition denote_restarts {E} `{schedulerE instruction_id_t -< E}
     : ktree E (list instruction_id_t) unit :=
-    ITree.iter (fun restarts =>
-                  match restarts with
-                  | [] => ret (inr tt)
-                  | riid::restarts =>
-                    trigger (Kill riid)
-                    ;; trigger (Spawn riid)
-                    ;; ret (inl restarts)
-                  end).
+    fun iids =>
+      'tt <- trigger (Kill iids)
+      ;; ITree.iter (fun respawn =>
+                       match respawn with
+                       | [] => ret (inr tt)
+                       | iid::respawn =>
+                         'tt <- trigger (Spawn iid)
+                         ;; ret (inl respawn)
+                       end) iids.
 
   Definition lift_mem_read {E}
              `{threadE -< E} `{nondetFinE -< E}
              `{schedulerE instruction_id_t -< E}
-             (slc : Arc.mem_slc)
-    : itree E Arc.mem_slc_val :=
+             (slc : mem_slc)
+    : itree E mem_slc_val :=
     rids <- trigger (ThEInitMemLoadOps slc)
     ;; ITree.iter (fun rids => (* Reads that aren't fully satisfied yet. *)
                      match rids with
@@ -102,22 +99,24 @@ Module Denote (Arc : ArcSig).
                        ;; read <- choose [trigger (ThESatMemLoadOpForwarding rid);
                                         (restarts <- trigger (ThESatMemLoadOpStorage rid)
                                          ;; ret (true, restarts))]
-                       ;; '(is_sat, restarts) <- read
-                       ;; 'tt <- denote_restarts restarts
+                       ;; is_sat <- exclusive_block
+                                     ('(is_sat, restarts) <- read
+                                      ;; 'tt <- denote_restarts restarts
+                                      ;; ret is_sat)
                        ;; ret (inl (if (is_sat : bool) then
                                       List.remove Nat.eq_dec rid rids
                                     else rids))
                      end) rids.
 
   Definition lift_mem_write_fp {E} `{threadE -< E} `{nondetFinE -< E}
-             (slc : Arc.mem_slc)
+             (slc : mem_slc)
     : itree E unit :=
     trigger (ThEInitMemStoreOpFps slc).
 
   Definition lift_mem_write_val {E}
              `{threadE -< E} `{nondetFinE -< E}
              `{schedulerE instruction_id_t -< E}
-             (val : Arc.mem_slc_val)
+             (val : mem_slc_val)
     : itree E unit :=
     'tt <- trigger (ThEInstaMemStoreOpVals val)
     ;; wids <- trigger ThECommitStoreInstruction
@@ -128,8 +127,9 @@ Module Denote (Arc : ArcSig).
                        ;; ret (inr tt)
                      | _ =>
                        wid <- choose wids
-                       ;; restarts <- trigger (ThEPropagateStoreOp wid)
-                       ;; 'tt <- denote_restarts restarts
+                       ;; 'tt <- exclusive_block
+                                  (restarts <- trigger (ThEPropagateStoreOp wid)
+                                   ;; denote_restarts restarts)
                        ;; ret (inl (List.remove Nat.eq_dec wid wids))
                      end) wids.
 
@@ -139,12 +139,8 @@ Module Denote (Arc : ArcSig).
     : Arc.InsSem.memE ~> itree E :=
     fun _ e =>
       match e with
-      | Arc.InsSem.MemERead loc => (* FIXME: InsSem should use slc instead of loc *)
-        lift_mem_read {| Arc.location := loc;
-                         Arc.size := 1 |}
-      | Arc.InsSem.MemEWriteFP loc => (* FIXME: InsSem should use slc instead of loc *)
-        lift_mem_write_fp {| Arc.location := loc;
-                               Arc.size :=1 |}
+      | Arc.InsSem.MemERead slc => lift_mem_read slc
+      | Arc.InsSem.MemEWriteFP slc => lift_mem_write_fp slc
       | Arc.InsSem.MemEWriteVal val => lift_mem_write_val val
       end.
 
@@ -156,7 +152,7 @@ Module Denote (Arc : ArcSig).
       let h := case_ lift_regE lift_memE in
       interp h it.
 
-  Definition new_instruction {E}
+  Definition spawn_instruction {E}
              `{wrapE threadE instruction_id_t -< E} `{nondetFinE -< E}
     : ktree (schedulerE instruction_id_t +' E)
             instruction_id_t
@@ -164,14 +160,13 @@ Module Denote (Arc : ArcSig).
     fun iid =>
       let it : itree (threadE +' nondetFinE +' schedulerE instruction_id_t)
                      (Types.result unit unit) :=
-          ast <- trigger ThEInsFetchAndDecode
-          ;; next_iids <- trigger ThEInsNextLocs
-          ;; ITree.iter (fun next_iids =>
-                           match next_iids with
-                           | [] => ret (inr tt)
-                           | niid::next_ins => trigger (Spawn niid)
-                                            ;; ret (inl next_iids)
-                           end) next_iids
+          '(next_iids, ast) <- trigger ThEFetchAndDecodeOrRestart
+          ;; 'tt <- ITree.iter (fun next_iids =>
+                                 match next_iids with
+                                 | [] => ret (inr tt)
+                                 | niid::next_ins => trigger (Spawn niid)
+                                                   ;; ret (inl next_iids)
+                                 end) next_iids
           ;; 'tt <- resum_it _ (lift_ins_sem _ (Arc.InsSem.denote ast))
           ;; 'tt <- trigger ThEFinishIns
           ;; ret (Accept tt) in
@@ -182,46 +177,23 @@ Module Denote (Arc : ArcSig).
              `{wrapE threadE instruction_id_t -< E} `{nondetFinE -< E}
     : ktree E instruction_id_t (Types.result unit unit) :=
     fun iid =>
-      resum_it _ (scheduler Nat.eq_dec new_instruction
+      resum_it _ (scheduler Nat.eqb spawn_instruction
                             (fun r1 r2 => match r1, r2 with
                                        | Accept tt, Accept tt => Accept tt
                                        | _, _ => Reject tt
                                        end)
                             (Accept tt)
-                            [(iid, new_instruction iid)]).
-End Denote.
+                            [(iid, spawn_instruction iid)]
+                            None).
 
 (*******************************************************************************)
-
-Module State(Arc : ArcSig).
-  Module DenoteA := Denote Arc.
-
-  Record mem_read : Type :=
-    mk_mem_read { read_id : mem_read_id_t;
-                  read_fp : Arc.mem_slc;
-                  read_kind : Arc.InsSem.mem_read_kind }.
-
-  Record mem_reads_state :=
-    mk_mem_reads_state { rs_footprint : Arc.mem_slc;
-                         rs_reads : list mem_read;
-                         rs_unsat_slcs : list (list Arc.mem_slc);
-                         rs_reads_from : list (list (instruction_id_t * mem_write_id_t * Arc.mem_slc)) }.
-
-  Record mem_write : Type :=
-    mk_mem_write { write_id : mem_write_id_t;
-                   write_fp : Arc.mem_slc;
-                   write_val : Arc.mem_slc_val;
-                   write_kind : Arc.InsSem.mem_read_kind }.
-
-  Record mem_writes_state :=
-    mk_mem_writes_state { ws_fps : list Arc.mem_slc;
-                          ws_writes : list mem_write;
-                          ws_has_propagated : list bool }.
+(** State **********************************************************************)
+(*******************************************************************************)
 
   Record reg_read_state :=
     mk_reg_read_state { rrs_slc : Arc.InsSem.reg_slc;
                         rrs_feeding_addr : bool;
-                        rrs_read_from : list (instruction_id_t * nat)
+                        rrs_reads_from : list (instruction_id_t * nat);
                                              (* the [nat] is an index into [ins_reg_writes.rws_slc]
                                                 of the instruction pointed by the [instruction_id_t]. *)
                         rrs_val : option Arc.InsSem.reg_val }.
@@ -229,49 +201,84 @@ Module State(Arc : ArcSig).
   Record reg_write_state :=
     mk_reg_write_state { rws_slc : Arc.InsSem.reg_slc;
                          rws_val : option Arc.InsSem.reg_val;
-                         (* [rws_deps] is a concatination of all the
-                            [rrs_read_from] of the instruction, when the
+                         (* [rws_reg_data_flow] is a concatination of all the
+                            [rrs_reads_from] of the instruction, when the
                             reg-write was performed. We assume that there is a
-                            dataflow from those to this reg-write, and therefore
+                            data-flow from those to this reg-write, and therefore
                             a dependency between the feeding instructions and
                             any instruction that reads from this
                             register-write. *)
-                         rws_deps : list (instruction_id_t * nat);
-                         rws_load_dep : bool }.
+                         rws_reg_data_flow : list (instruction_id_t * nat);
+                         (* [rws_mem_data_flow] indicates if the instruction has
+                            performed a memory read before the reg-write. If so,
+                            we assume that there is a data-flow from the memory
+                            to this reg-write. *)
+                         rws_mem_data_flow : bool }.
+
+  Record mem_read : Type :=
+    mk_mem_read { read_id : mem_read_id_t;
+                  read_footprint : mem_slc;
+                  read_kind : Arc.InsSem.mem_read_kind }.
+
+  (* [mem_read_value] is actually a pointer to all the sources that compose the
+     value *)
+  Definition mem_read_value : Type := list (thread_id_t * instruction_id_t * mem_write_id_t *
+                                            mem_slc * mem_slc_val).
+
+  Record mem_reads_state :=
+    mk_mem_reads_state { rs_footprint : mem_slc;
+                         rs_reads : list mem_read;
+                         rs_unsat_slcs : list (list mem_slc);
+                         rs_reads_from : list mem_read_value }.
+
+  Instance eta_mem_reads_state : Settable _ :=
+    settable! mk_mem_reads_state <rs_footprint; rs_reads; rs_unsat_slcs; rs_reads_from>.
+
+  Record mem_write : Type :=
+    mk_mem_write { write_id : mem_write_id_t;
+                   write_fp : mem_slc;
+                   write_val : mem_slc_val;
+                   write_kind : Arc.InsSem.mem_read_kind }.
+
+  Record mem_writes_state :=
+    mk_mem_writes_state { ws_footprint : mem_slc;
+                          ws_writes : list mem_write;
+                          ws_has_propagated : list bool }.
+
+  Instance eta_mem_writes_state : Settable _ :=
+    settable! mk_mem_writes_state <ws_footprint; ws_writes; ws_has_propagated>.
 
   Record decoded_instruction_state :=
     mk_decoded_instruction_state {
+        ins_ast : Arc.InsSem.ast;
         (* statically analysed data about the instruction*)
-        ins_kind: Arc.instruction_kind;
+        ins_kind : Arc.instruction_kind;
 
-        ins_reg_reads : list reg_reads_state;
-        ins_reg_writes : list reg_writes_state;
+        ins_reg_reads : list reg_read_state;
+        ins_reg_writes : list reg_write_state;
 
-        reg_writes: list (Arc.InsSem.reg_ * (list register_write_dependency * register_value));
+        ins_mem_reads : option mem_reads_state;
+        ins_mem_writes : option mem_writes_state;
 
-        ins_mem_reads: option mem_reads_state;
-        ins_mem_writes: option mem_writes_state;
-
-        ins_finished: bool }.
+        ins_finished : bool }.
 
   Instance eta_decoded_instruction_state : Settable _ :=
-    settable! mk_decoded_instruction_state <ins_kind; ins_regs_in; ins_regs_feeding_address; ins_regs_out; ins_mem_reads; ins_mem_writes; ins_finished>.
+    settable! mk_decoded_instruction_state <ins_ast; ins_kind; ins_reg_reads; ins_reg_writes; ins_mem_reads; ins_mem_writes; ins_finished>.
 
   Definition initial_decoded_instruction_state
              (ast : Arc.InsSem.ast)
     : decoded_instruction_state :=
-    let '(regs_in, regs_feeding_address, regs_out) := Arc.InsSem.regs_from_ast ast in
-    (* instruction_state: *)
-    {| ins_kind := (Arc.instruction_kind_from_ast ast);
-       ins_regs_in := regs_in;
-       ins_regs_feeding_address := regs_feeding_address;
-       ins_regs_out := regs_out;
+    let '(regs_in, regs_out) := Arc.InsSem.regs_from_ast ast in
+    {| ins_ast := ast;
+       ins_kind := (Arc.instruction_kind_from_ast ast);
+       ins_reg_reads := List.map (fun '(slc, addr) => mk_reg_read_state slc addr [] None) regs_in;
+       ins_reg_writes := List.map (fun slc => mk_reg_write_state slc None [] false) regs_out;
        ins_mem_reads := None;
        ins_mem_writes := None;
        ins_finished := false |}.
 
   Definition instruction_state : Type := instruction_id_t *
-                                         Arc.mem_loc *
+                                         mem_loc *
                                          option decoded_instruction_state.
 
   Record state :=
@@ -281,147 +288,208 @@ Module State(Arc : ArcSig).
   Instance eta_state : Settable _ :=
     settable! mk_state <next_iid; instruction_tree>.
 
-  Definition initial_state (loc : Arc.mem_loc)
+  Definition initial_state (iid : instruction_id_t) (loc : mem_loc)
     : state :=
-    {| next_iid := 1;
-       instruction_tree := Tree (0, loc, None) [] |}.
+    {| next_iid := iid + 1;
+       instruction_tree := Tree (iid, loc, None) [] |}.
 
   Variant storageE : Type -> Type :=
-  | StEReadInstruction : Arc.InsSem.pc_t -> storageE Arc.InsSem.machine_code
-  | StERead : mem_read_id_t -> storageE unit.
+  | StEReadInstruction : Arc.InsSem.pc_t -> storageE (mem_slc * mem_read_value)
+  | StERead : mem_read -> (list mem_slc) -> storageE mem_read_value
+  | StEWrite : mem_write -> storageE unit.
 
   Definition get_instruction_state {E} `{exceptE error -< E}
              (iid : instruction_id_t) (s : state)
-    : itree E instruction_state :=
-    let fix helper t :=
-        let '(Tree ((iid', _, _) as i) ts) := t in
-        if Nat.eqb iid' iid then Some i
+    : itree E (list instruction_state * instruction_state * list (tree instruction_state)) :=
+    let fix helper prefix t :=
+        let '(Tree ((iid', _, _) as i) subts) := t in
+        if Nat.eqb iid' iid then Some (prefix, i, subts)
         else
           match List.find (fun x => match x with None => false | _ => true end)
-                          (List.map helper ts) with
+                          (List.map (helper (i::prefix)) subts) with
           | Some x => x
           | None => None
           end
     in
-    try_unwrap_option (helper s.(instruction_tree)) "get_instruction_state: Can't find iid".
+    try_unwrap_option (helper [] s.(instruction_tree)) "get_instruction_state: Can't find iid".
 
   Definition get_dec_instruction_state {E} `{exceptE error -< E}
              (iid : instruction_id_t) (s : state)
-    : itree E decoded_instruction_state :=
-    '(_, _, ins) <- get_instruction_state iid s
-    ;; try_unwrap_option ins "get_dec_instruction_state: instruction was not decoded yet".
+    : itree E (list instruction_state * decoded_instruction_state * list (tree instruction_state)) :=
+    '(prefix, (_, _, ins), subts) <- get_instruction_state iid s
+    ;; dins <- try_unwrap_option ins "get_dec_instruction_state: instruction was not decoded yet"
+    ;; ret (prefix, dins, subts).
 
-  Definition update_dec_instruction_state (iid : instruction_id_t)
-             (ins : decoded_instruction_state) (s : state)
+  Definition update_dec_instruction_state_and_subts
+             (iid : instruction_id_t) (dins : decoded_instruction_state)
+             (subts : list (tree instruction_state)) (s : state)
     : state :=
     let fix helper t :=
-        let '(Tree ((iid', loc, _) as i) ts) := t in
-        if Nat.eqb iid' iid then Tree (iid, loc, Some ins) ts
-        else Tree i (List.map helper ts)
+        let '(Tree ((iid', loc, _) as i) subts') := t in
+        if Nat.eqb iid' iid then Tree (iid, loc, Some dins) subts
+        else Tree i (List.map helper subts')
     in
     s <| instruction_tree := helper s.(instruction_tree) |>.
+
+  Definition update_dec_instruction_state
+             (iid : instruction_id_t) (dins : decoded_instruction_state)
+             (s : state)
+    : state :=
+    let fix helper t :=
+        let '(Tree ((iid', loc, _) as i) subts) := t in
+        if Nat.eqb iid' iid then Tree (iid, loc, Some dins) subts
+        else Tree i (List.map helper subts)
+    in
+    s <| instruction_tree := helper s.(instruction_tree) |>.
+
+  Definition try_fetch_and_decode_or_restart {E} `{storageE -< E} `{exceptE error -< E}
+             (iid : instruction_id_t) (s : state)
+    : itree E (state * (list instruction_id_t * Arc.InsSem.ast)) :=
+    '(_, (_, loc, ins), _) <- get_instruction_state iid s
+    ;; match ins with
+       | None =>
+         '(slc, vals) <- trigger (StEReadInstruction loc)
+         ;; let vals := List.map (fun '(_, _, _, s, v) => (s, v)) vals in
+            val <- try_unwrap_option (flatten_mem_slc_vals slc vals)
+                                    "try_fetch_and_decode_or_restart: some bytes are missing from memory read of instruction."
+         ;; let ast := Arc.InsSem.decode (nat_of_mem_slc_val val) in
+            let ins := initial_decoded_instruction_state ast in
+            let next_pcs := Arc.InsSem.next_pc loc ast in
+            let iids := List.seq s.(next_iid) (List.length next_pcs) in
+            let subts := List.map (fun '(iid, pc) => Tree (iid, pc, None) [])
+                                  (List.combine iids next_pcs) in
+            let s := s <| next_iid := s.(next_iid) + (List.length next_pcs) |> in
+            let s := update_dec_instruction_state_and_subts iid ins subts s in
+            ret (s, (iids, ast))
+       | Some ins =>
+         (* Nothing to do, the instruction-state has already been restarted. *)
+         ret (s, ([], ins.(ins_ast)))
+       end.
+
+  Definition try_finish_instruction {E} `{exceptE error -< E}
+             (iid : instruction_id_t) (s : state)
+    : itree E (state * unit) :=
+    (* FIXME: check finish condition *)
+    ret (s, tt).
 
   Definition try_read_reg_slc {E}
              (rslc : Arc.InsSem.reg_slc) (iid : instruction_id_t) (s : state)
     : itree E (state * Arc.InsSem.reg_val) :=
     ITree.spin.
 
-  Definition try_write_reg_slc {E}
+  Definition try_write_reg_slc {E} `{exceptE error -< E}
              (rslc : Arc.InsSem.reg_slc) (val : Arc.InsSem.reg_val)
              (iid : instruction_id_t) (s : state)
     : itree E (state * unit) :=
-    ins <- get_dec_instruction_state iid s
-    ;; update_dec_instruction_state iid () s
-
-  Definition handle_reg_access {E} `{exceptE error -< E}
-             {A} (e : Arc.InsSem.regE A) (iid : instruction_id_t) (s : state)
-    : itree E (state * A) :=
-    match e with
-    | Arc.InsSem.RegERead rslc => try_read_reg_slc rslc iid s
-    | Arc.InsSem.RegEWrite rslc rval => try_write_reg_slc rslc rval iid s
-    end.
-
-  Definition try_fetch_and_decode {E} `{storageE -< E} `{exceptE error -< E}
-             (iid : instruction_id_t) (s : state)
-    : itree E (state * Arc.InsSem.ast) :=
-    '(_, loc, _) <- get_instruction_state iid s
-    ;; mem_read_result <- trigger (StEReadInstruction loc)
-    ;; code <- value_from_mem_read_result mem_read_result
-    ;; ast <- Arc.InsSem.decode code
-    ;; let ins := initial_decoded_instruction_state ast in
+    '(_, ins, _) <- get_dec_instruction_state iid s
+    ;; let reg_writes :=
+           List.map
+             (fun rws =>
+                if Arc.InsSem.reg_slc_eqb rws.(rws_slc) rslc then
+                  let rdf := List.concat (List.map rrs_reads_from ins.(ins_reg_reads)) in
+                  let mdf := match ins.(ins_mem_reads) with Some _ => true | _ => false end in
+                  mk_reg_write_state rslc (Some val) rdf mdf
+                else rws)
+             ins.(ins_reg_writes) in
+       let ins := ins <| ins_reg_writes := reg_writes |> in
        let s := update_dec_instruction_state iid ins s in
-       ret (s, ast).
-
-  Definition try_get_next_locations {E} `{exceptE error -< E}
-             (iid : instruction_id_t) (s : state)
-    : itree E (state * list instruction_id_t) :=
-    iic <- get_instruction_in_context iid s
-    ;; ins <- get_decoded_instruction_state iic
-    ;; let next_pcs := Arc.InsSem.next_pc ins.(ins_loc) ins.(ins_ast) in
-       let iids := List.seq s.(next_iid) (List.length next_pcs) in
-       let iidpcs := List.combine iids next_pcs in
-       let new_subtrees := List.map (fun (iid, pc) => Tree (ISUnfetched pc) []) iidpcs in
-       let s := s <| next_iid := s.(next_iid) + (List.length next_pcs) |>
-                  <| instruction_tree := apply_tree_context iic.(iic_context) iic.(iic_instruction) new_subtrees |> in
-       ret (s, iids).
-
-  Definition try_init_mem_load_ops {E} `{exceptE error -< E}
-             (slc : Arc.mem_slc) (iid : instruction_id_t) (s : state)
-    : itree E (state * list mem_read_id_t) :=
-    throw NotImplemented.
-
-  Definition try_write_forward {E} `{exceptE error -< E}
-             (rid : mem_read_id_t) (iid : instruction_id_t) (s : state)
-    : itree E (state * bool) :=
-    throw NotImplemented.
-
-  Definition try_sat_mem_load_op_from_storage {E} `{storageE -< E} `{exceptE error -< E}
-             (rid : mem_read_id_t) (iid : instruction_id_t) (s : state)
-    : itree E (state * unit) :=
-    iic <- get_instruction_in_context iid s
-    ;; ins <- get_decoded_instruction_state iic
-    ;; rr <- get_mem_read_request rid ins
-    ;; mem_read_result <- trigger (StoERead rr)
-    ;; ins <- update_mem_read_request mem_read_result rid ins
-    ;; let s := <| instruction_tree := apply_tree_context iic.(iic_context) (ISDecoded ins) iic.(iic_subtrees) |> in
        ret (s, tt).
 
-  Definition try_complete_load_ops {E} `{exceptE error -< E}
+  Definition handle_reg_access {E} `{exceptE error -< E}
+             (iid : instruction_id_t)
+    : Arc.InsSem.regE ~> stateT state (itree E) :=
+    fun _ e s =>
+      match e with
+      | Arc.InsSem.RegERead rslc => try_read_reg_slc rslc iid s
+      | Arc.InsSem.RegEWrite rslc rval => try_write_reg_slc rslc rval iid s
+      end.
+
+  Definition try_init_mem_load_ops {E} `{exceptE error -< E}
+             (slc : mem_slc) (iid : instruction_id_t) (s : state)
+    : itree E (state * list mem_read_id_t) :=
+    '(_, ins, _) <- get_dec_instruction_state iid s
+    ;; let sub_slcs := Arc.split_load_mem_slc ins.(ins_kind) slc in
+       let kind := Arc.mem_read_kind_of_ins_kind ins.(ins_kind) in
+       let rids := List.seq 0 (List.length sub_slcs) in
+       let reads := List.map
+                      (fun '(rid, slc) => {| read_id := rid;
+                                          read_footprint := slc;
+                                          read_kind := kind |})
+                      (List.combine rids sub_slcs) in
+       let rs := {| rs_footprint := slc;
+                    rs_reads := reads;
+                    rs_unsat_slcs := List.map (fun r => [r.(read_footprint)]) reads;
+                    rs_reads_from := List.map (fun _ => nil) reads |} in
+       let ins := ins <| ins_mem_reads := Some rs |> in
+       let s := update_dec_instruction_state iid ins s in
+       ret (s, rids).
+
+
+  Definition try_sat_mem_load_op_forwarding {E} `{exceptE error -< E} `{exceptE disabled -< E}
+             (rid : mem_read_id_t) (iid : instruction_id_t) (s : state)
+    : itree E (state * (bool * list instruction_id_t)) :=
+    (* FIXME: *)
+    ITree.spin.
+
+  Definition try_sat_mem_load_op_from_storage {E}
+             `{storageE -< E} `{exceptE error -< E} `{exceptE disabled -< E}
+             (rid : mem_read_id_t) (iid : instruction_id_t) (s : state)
+    : itree E (state * list instruction_id_t) :=
+    '(_, ins, subts) <- get_dec_instruction_state iid s
+    ;; rs <- try_unwrap_option ins.(ins_mem_reads)
+                                    "try_sat_mem_load_op_from_storage: no reads."
+    ;; unsat_slcs <- try_unwrap_option (List.nth_error rs.(rs_unsat_slcs) rid)
+                                      "try_sat_mem_load_op_from_storage: missing rid."
+    ;; guard (isTrue (unsat_slcs <> []))
+    ;; rr <- try_unwrap_option (List.nth_error rs.(rs_reads) rid)
+                              "try_sat_mem_load_op_from_storage: missing rid"
+    ;; rf_forward <- try_unwrap_option (List.nth_error rs.(rs_reads_from) rid)
+                                      "try_sat_mem_load_op_from_storage: missing rid."
+    ;; rf_storage <- trigger (StERead rr unsat_slcs)
+    ;; let rs := rs <| rs_unsat_slcs := list_replace_nth rid [] rs.(rs_unsat_slcs) |>
+                    <| rs_reads_from := list_replace_nth rid (rf_forward ++ rf_storage) rs.(rs_reads_from) |> in
+       let ins := ins <| ins_mem_reads := Some rs |> in
+       (* FIXME: compute iids that need to be restarted *)
+       let restarts : list instruction_id_t := [] in
+       (* FIXME: let subts := restart_instructions restarts subts in *)
+       let s := update_dec_instruction_state_and_subts iid ins subts s in
+       ret (s, restarts).
+
+  Definition try_complete_load_ops {E} `{exceptE error -< E} `{exceptE disabled -< E}
              (iid : instruction_id_t) (s : state)
     : itree E (state * mem_slc_val) :=
-    iic <- get_instruction_in_context iid s
-    ;; ins <- get_decoded_instruction_state iic
-    ;; val <- get_mem_reads_value ins
+    '(_, ins, _) <- get_dec_instruction_state iid s
+    ;; rs <- try_unwrap_option ins.(ins_mem_reads)
+                                    "try_complete_load_ops: no reads."
+    ;; guard (isTrue (Forall (fun u => u = []) rs.(rs_unsat_slcs)))
+    ;; val <- try_unwrap_option
+               (flatten_mem_slc_vals
+                  rs.(rs_footprint)
+                       (List.concat (List.map
+                                       (List.map (fun '(_, _, _, s, v) => (s, v)))
+                                       rs.(rs_reads_from))))
+               "try_complete_load_ops: some bytes are missing from memory read."
     ;; ret (s, val).
 
-  Definition try_finish_instruction {E} `{exceptE error -< E}
-             (iid : instruction_id_t) (s : state)
-    : itree E (state * unit) :=
-    throw NotImplemented.
-
-  Definition handle_threadE {E} `{storageE -< E} `{exceptE error -< E}
-    : wrapE ThrDenote.threadE Thread.instruction_id_t ~>
+  Definition handle_threadE {E} `{storageE -< E} `{exceptE error -< E} `{exceptE disabled -< E}
+    : wrapE threadE instruction_id_t ~>
             stateT state (itree E) :=
     fun _ e s =>
       let '(Wrap e iid) := e in
       match e with
-      | ThEInsFetchAndDecode => try_fetch_and_decode iid s
-      | ThEInsNextLocs => try_get_next_locations iid s
+      | ThEFetchAndDecodeOrRestart => try_fetch_and_decode_or_restart iid s
       | ThEFinishIns => try_finish_instruction iid s
-      | ThERegAccess _ e => handle_reg_access e iid s
+      | ThERegAccess _ e => handle_reg_access iid _ e s
       (* Load events *)
       | ThEInitMemLoadOps slc => try_init_mem_load_ops slc iid s
-      | ThESatMemLoadOpForwarding rid => throw NotImplemented
+      | ThESatMemLoadOpForwarding rid => try_sat_mem_load_op_forwarding rid iid s
       | ThESatMemLoadOpStorage rid => try_sat_mem_load_op_from_storage rid iid s
       | ThECompleteLoadOps => try_complete_load_ops iid s
       (* Store events *)
-      (* | ThEInitMemStoreOpFps : Arc.mem_slc -> threadE unit *)
-      (* | ThEInstaMemStoreOpVals : Arc.mem_slc_val -> threadE unit *)
-      (* | ThECommitStoreInstruction : threadE (list mem_write_id_t) *)
-      (* | ThEPropagateStoreOp : mem_write_id_t -> threadE unit *)
-      (* | ThECompleteStoreOps : threadE unit. *)
+      | ThEInitMemStoreOpFps slc => ITree.spin (* : mem_slc -> threadE unit *)
+      | ThEInstaMemStoreOpVals val => ITree.spin (* mem_slc_val -> threadE unit *)
+      | ThECommitStoreInstruction => ITree.spin (* threadE (list mem_write_id_t) *)
+      | ThEPropagateStoreOp wid => ITree.spin (* mem_write_id_t -> threadE unit *)
+      | ThECompleteStoreOps => ITree.spin (* threadE unit *)
       end.
-
-
-
-End State.
+End Make.
