src/Types.v
@@ -6,7 +6,7 @@ From Coq Require Import
      Strings.String
      Morphisms
      Setoid
-     RelationClasses .
+     RelationClasses.
 
 (* From ExtLib Require Import *)
 (*      Data.String *)
@@ -34,12 +34,23 @@ Local Open Scope itree_scope.
    This bounds the instance search depth: *)
 Typeclasses eauto := 5.
 
+From RecordUpdate Require Import RecordSet.
+Import RecordSetNotations.
+
+Require Import Utils.
+Require Import Decision.
+
 (* [throw Disabled] indicates a disabled transition, backtrack and try a
    different non-det choice. It is intended that [Disabled] can only happen
    immediately after a non-det choice; and whenever there is a non-det option,
    at least one of the choices is not [Disabled]. Hence non-det options can
    easily be pruned to not include [Disabled] deadlocks. *)
 Variant disabled : Type := Disabled : disabled.
+
+Definition guard {E} `{exceptE disabled -< E}
+           (p : bool) : itree E unit :=
+  if p then Ret tt
+  else throw Disabled.
 
 (* Indicates a bug in the model *)
 Variant error : Type := Error : string -> error.
@@ -58,13 +69,66 @@ Variant result A R : Type :=
 Arguments Accept {A R}.
 Arguments Reject {A R}.
 
+Definition thread_id_t := Utils.id_t.
+Definition instruction_id_t := Utils.id_t.
+Definition mem_read_id_t := Utils.id_t.
+Definition mem_write_id_t := Utils.id_t.
+
+Definition mem_loc : Type := nat.
+Record mem_slc : Type :=
+  mk_mem_slc { location : mem_loc;
+               size : nat (* in bytes *) }.
+(* [mem_slc_val] is a list of byte values, head is least significant. *)
+Definition mem_slc_val : Type := list nat.
+
+Definition flatten_mem_slc_vals (slc : mem_slc) (vals : list (mem_slc * mem_slc_val))
+  : option mem_slc_val :=
+  let byte_locs := List.seq slc.(location) slc.(size) in
+  let byte_of_val slc val (loc : nat) :=
+      if decide (slc.(location) <= loc < (slc.(location) + slc.(size))) then
+        List.nth_error val (loc - slc.(location))
+      else None in
+  let fix byte_of_vals vals loc :=
+      match vals with
+      | (slc', val')::vals' =>
+        match byte_of_val slc' val' loc with
+        | Some b => Some b
+        | None => byte_of_vals vals' loc
+        end
+      | [] => None
+      end in
+  let bytes := List.map (byte_of_vals vals) byte_locs in
+  List.fold_left (fun acc b =>
+                    match acc, b with
+                    | Some acc, Some b => Some (b::acc)
+                    | _, _ => None
+                    end)
+                 bytes
+                 (Some nil).
+
+Definition nat_of_mem_slc_val (val : mem_slc_val) : nat :=
+  List.fold_left
+    (fun acc b => (Nat.shiftl acc 8) + b)
+    (List.rev val) 0.
+
+Definition mem_slc_val_of_nat (val : nat) (size : nat) : mem_slc_val :=
+  List.map
+    (fun off => Nat.land (2 ^ 8 - 1) (Nat.shiftr val (8 * off)))
+    (List.seq 0 size).
+
 Module Type InstructionSemanticsSig.
   Variable reg : Type.
+  Variable reg_eqb : reg -> reg -> bool.
   Variable reg_size : reg -> nat.
 
   (* `(a,b)` represents all the bits between `a` and `b`, including `a` but not
   including `b`. *)
   Definition reg_slc : Type := reg * (nat * nat).
+  Definition reg_slc_eqb (s1 s2 : reg_slc) : bool :=
+    let '(r1, (a1, b1)) := s1 in
+    let '(r2, (a2, b2)) := s2 in
+    reg_eqb r1 r2 && Nat.eqb a1 a2 && Nat.eqb b1 b2.
+
   Definition reg_val : Type := N.
 
   Variable mem_read_kind : Type.
@@ -73,16 +137,16 @@ Module Type InstructionSemanticsSig.
   Variable ast : Type.
 
   Variable regs_from_ast
-    : ast -> (ListSet.set reg_slc * ListSet.set reg_slc * ListSet.set reg_slc).
+    : ast -> (list (reg_slc * bool) * list reg_slc).
 
   Variant regE : Type -> Type :=
   | RegERead : reg_slc -> regE reg_val
   | RegEWrite : reg_slc -> reg_val -> regE unit.
 
   Variant memE : Type -> Type :=
-  | MemERead : nat -> memE nat
-  | MemEWriteFP (loc : nat) : memE unit
-  | MemEWriteVal (val : nat) : memE unit.
+  | MemERead : mem_slc -> memE mem_slc_val
+  | MemEWriteFP : mem_slc -> memE unit
+  | MemEWriteVal : mem_slc_val -> memE unit.
 
   Definition E := (regE +' memE).
 
@@ -98,15 +162,14 @@ End InstructionSemanticsSig.
 Module Type ArcSig.
   Declare Module InsSem : InstructionSemanticsSig.
 
-  Definition mem_loc := nat.
-  Record mem_slc : Type :=
-    mk_mem_slc { location : mem_loc;
-                 size : nat (* in bytes *) }.
-  Definition mem_slc_val : Type := nat.
-
   Variable instruction_kind : Type.
   Variable instruction_kind_from_ast : InsSem.ast -> instruction_kind.
-  (* Variable instruction_semantics_state : Type. *)
+
+  Variable split_load_mem_slc : instruction_kind -> mem_slc -> list mem_slc.
+  Variable split_store_mem_slc : instruction_kind -> mem_slc -> list mem_slc.
+
+  Variable mem_read_kind_of_ins_kind : instruction_kind -> InsSem.mem_read_kind.
+  Variable mem_write_kind_of_ins_kind : instruction_kind -> InsSem.mem_read_kind.
 End ArcSig.
 
 Module Type ThreadSig.
